update

theory/Static_Framework.thy
@@ -13,7 +13,7 @@ type_synonym node_set = "node_label set"
 
 type_synonym node_map = "node_label \<Rightarrow> var set"
 
-datatype edge_label = ENext | ESpawn (* | ESend var | ECall var | EReturn var *)
+datatype edge_label = ENext | ESpawn | ECall | EReturn
 
 type_synonym flow_label = "(node_label \<times> edge_label \<times> node_label)"
 
@@ -168,6 +168,443 @@ proof -
     using is_super_exp1 is_super_exp_trans by blast
   qed
 qed
+
+
+inductive is_super_exp_over_prim :: "exp \<Rightarrow> prim \<Rightarrow> bool" where
+  Send_Evt: "
+    is_super_exp_over_prim e0 (Send_Evt xC xM)
+  " |
+  Recv_Evt: "
+    is_super_exp_over_prim e0 (Recv_Evt xC)
+  " |
+  Pair: "
+    is_super_exp_over_prim e0 (Pair x1 x2)
+  " |
+  Left: "
+    is_super_exp_over_prim e0 (Left x)
+  " |
+  Right: "
+    is_super_exp_over_prim e0 (Right x)
+  " |
+  Abs: "
+    is_super_exp_left e0 e\<^sub>b \<Longrightarrow>
+    is_super_exp_over_prim e0 (Abs f\<^sub>p x\<^sub>p e\<^sub>b)
+  " 
+
+inductive 
+  is_super_exp_over_env :: "exp \<Rightarrow> val_env \<Rightarrow> bool" and
+  is_super_exp_over_val :: "exp \<Rightarrow> val \<Rightarrow> bool"
+where
+  VUnit: "
+    is_super_exp_over_val e0 VUnit
+  " |
+  VChan: "
+    is_super_exp_over_val e0 (VChan c)
+  " |
+  VClosure: "
+    is_super_exp_over_prim e0 p \<Longrightarrow>
+    is_super_exp_over_env e0 \<rho>' \<Longrightarrow>
+    is_super_exp_over_val e0 (VClosure p \<rho>')
+  " |
+
+  Intro: "
+    \<forall> x \<omega> . \<rho> x = Some \<omega> \<longrightarrow> is_super_exp_over_val e0 \<omega> \<Longrightarrow>
+    is_super_exp_over_env e0 \<rho>
+  "
+
+inductive is_super_exp_over_stack :: "exp \<Rightarrow> cont list \<Rightarrow> bool" where
+  Empty: "
+    is_super_exp_over_stack e0 []
+  " |
+  Nonempty: "
+    is_super_exp_left e0 e\<^sub>\<kappa> \<Longrightarrow>
+    is_super_exp_over_env e0 \<rho>\<^sub>\<kappa> \<Longrightarrow>
+    is_super_exp_over_stack e0 \<kappa> \<Longrightarrow>
+    is_super_exp_over_stack e0 (\<langle>x\<^sub>\<kappa>,e\<^sub>\<kappa>,\<rho>\<^sub>\<kappa>\<rangle> # \<kappa>)
+  "
+
+inductive is_super_exp_over_state :: "exp \<Rightarrow> state \<Rightarrow> bool" where
+  Intro: "
+    is_super_exp_left e0 e \<Longrightarrow>
+    is_super_exp_over_env e0 \<rho> \<Longrightarrow>
+    is_super_exp_over_stack e0 \<kappa> \<Longrightarrow>
+    is_super_exp_over_state e0 (\<langle>e;\<rho>;\<kappa>\<rangle>)
+  "
+
+lemma is_super_exp_over_state_preserved: "
+  (E, H) \<rightarrow> (E', H') \<Longrightarrow>
+  \<forall>\<pi> \<sigma>. E \<pi> = Some \<sigma> \<longrightarrow> is_super_exp_over_state e\<^sub>0 \<sigma> \<Longrightarrow>
+  E' \<pi>' = Some \<sigma>' \<Longrightarrow>
+  is_super_exp_over_state e\<^sub>0 \<sigma>'
+"
+proof -
+  assume 
+    H1: "\<forall>\<pi> \<sigma>. E \<pi> = Some \<sigma> \<longrightarrow> is_super_exp_over_state e\<^sub>0 \<sigma>" and
+    H2: "E' \<pi>' = Some \<sigma>'" and
+    H3: "(E, H) \<rightarrow> (E', H')"
+
+  from H3 show "is_super_exp_over_state e\<^sub>0 \<sigma>'"
+  proof cases
+    case (Seq_Step_Down \<pi> x \<rho> x\<^sub>\<kappa> e\<^sub>\<kappa> \<rho>\<^sub>\<kappa> \<kappa> \<omega>)
+
+    from H1 local.Seq_Step_Down(4)
+    have L1H1: "is_super_exp_over_state e\<^sub>0 (\<langle>RESULT x;\<rho>;\<langle>x\<^sub>\<kappa>,e\<^sub>\<kappa>,\<rho>\<^sub>\<kappa>\<rangle> # \<kappa>\<rangle>)" by blast
+
+    then have 
+      L1H2: "is_super_exp_over_env e\<^sub>0 \<rho>" and 
+      L1H3: "is_super_exp_over_stack e\<^sub>0 (\<langle>x\<^sub>\<kappa>,e\<^sub>\<kappa>,\<rho>\<^sub>\<kappa>\<rangle> # \<kappa>)" by (blast dest: is_super_exp_over_state.cases)+
+
+    then have 
+      L1H4: "is_super_exp_left e\<^sub>0 e\<^sub>\<kappa>" and 
+      L1H5: "is_super_exp_over_env e\<^sub>0 \<rho>\<^sub>\<kappa>" and 
+      L1H6: "is_super_exp_over_stack e\<^sub>0 \<kappa>" by (blast dest: is_super_exp_over_stack.cases)+
+
+    from L1H2 L1H5 local.Seq_Step_Down(5) have L1H7: "is_super_exp_over_env e\<^sub>0 (\<rho>\<^sub>\<kappa>(x\<^sub>\<kappa> \<mapsto> \<omega>))"
+      by (smt is_super_exp_over_env.cases is_super_exp_over_env_is_super_exp_over_val.Intro map_upd_Some_unfold)
+
+    with L1H4 L1H6 L1H7 have L1H8: "is_super_exp_over_state e\<^sub>0 (\<langle>e\<^sub>\<kappa>;\<rho>\<^sub>\<kappa>(x\<^sub>\<kappa> \<mapsto> \<omega>);\<kappa>\<rangle>)"
+      by (simp add: is_super_exp_over_state.intros)
+
+    with H1 H2 local.Seq_Step_Down(1) show "is_super_exp_over_state e\<^sub>0 \<sigma>'"
+      by (metis map_add_empty map_add_upd map_upd_Some_unfold)
+  next
+    case (Seq_Step \<pi> x b el \<rho>l \<kappa>l \<omega>)
+
+    from H1 local.Seq_Step(4) 
+    have L1H1: "is_super_exp_over_state e\<^sub>0 (\<langle>LET x = b in el;\<rho>l;\<kappa>l\<rangle>)" by blast
+
+    then have 
+      L1H2: "is_super_exp_left e\<^sub>0 (LET x = b in el)" and
+      L1H3: "is_super_exp_over_env e\<^sub>0 \<rho>l" and
+      L1H4: "is_super_exp_over_stack e\<^sub>0 \<kappa>l" by (blast dest: is_super_exp_over_state.cases)+
+
+    from L1H2 have L1H5: "is_super_exp_left e\<^sub>0 el" by (blast dest: is_super_exp_left.Let)
+
+    from local.Seq_Step(5) have 
+      "is_super_exp_over_val e\<^sub>0 \<omega>"
+    proof cases
+      case Let_Unit
+      then show "is_super_exp_over_val e\<^sub>0 \<omega>" by (simp add: VUnit)
+    next
+      case (Let_Prim p)
+
+      have L2H1: "is_super_exp_over_prim e\<^sub>0 p"
+      proof (cases p)
+        case (Send_Evt x11 x12)
+        then show "is_super_exp_over_prim e\<^sub>0 p" by (simp add: is_super_exp_over_prim.Send_Evt)
+      next
+        case (Recv_Evt x2)
+        then show "is_super_exp_over_prim e\<^sub>0 p" by (simp add: is_super_exp_over_prim.Recv_Evt)
+      next
+        case (Pair x31 x32)
+        then show "is_super_exp_over_prim e\<^sub>0 p" by (simp add: is_super_exp_over_prim.Pair)
+      next
+        case (Left x4)
+        then show "is_super_exp_over_prim e\<^sub>0 p" by (simp add: is_super_exp_over_prim.Left)
+      next
+        case (Right x5)
+        then show "is_super_exp_over_prim e\<^sub>0 p" by (simp add: is_super_exp_over_prim.Right)
+      next
+        case (Abs x61 x62 x63)
+
+        with L1H2 local.Let_Prim(1) local.Abs
+        show "is_super_exp_over_prim e\<^sub>0 p" by (smt is_super_exp_left.Let_Abs_Body is_super_exp_over_prim.Abs )
+      qed
+
+      have L2H3: "is_super_exp_over_env e\<^sub>0 \<rho>l" by (simp add: L1H3)
+
+      with L2H1 have "is_super_exp_over_val e\<^sub>0 (VClosure p \<rho>l)" by (simp add: VClosure)
+
+      with local.Let_Prim(2) show "is_super_exp_over_val e\<^sub>0 \<omega>" by simp
+    next
+      case (Let_Fst x\<^sub>p x\<^sub>1 x\<^sub>2 \<rho>\<^sub>p)
+      then show "is_super_exp_over_val e\<^sub>0 \<omega>"
+        by (metis L1H3 is_super_exp_over_env.cases is_super_exp_over_val.cases val.distinct(3) val.distinct(5) val.inject(2))
+    next
+      case (Let_Snd x\<^sub>p x\<^sub>1 x\<^sub>2 \<rho>\<^sub>p)
+      then show "is_super_exp_over_val e\<^sub>0 \<omega>"
+        by (metis L1H3 is_super_exp_over_env.cases is_super_exp_over_val.cases val.distinct(3) val.distinct(5) val.inject(2))
+    qed
+    
+    with L1H3 have L1H6: "is_super_exp_over_env e\<^sub>0 (\<rho>l(x \<mapsto> \<omega>))"
+      by (smt is_super_exp_over_env.cases is_super_exp_over_env_is_super_exp_over_val.Intro map_upd_Some_unfold)
+
+    with L1H4 L1H5 have L1H7: "is_super_exp_over_state e\<^sub>0 (\<langle>el;\<rho>l(x \<mapsto> \<omega>);\<kappa>l\<rangle>)" by (simp add: is_super_exp_over_state.intros)
+   
+    with H1 H2 local.Seq_Step(1) show "is_super_exp_over_state e\<^sub>0 \<sigma>'"
+      by (metis map_add_empty map_add_upd map_upd_Some_unfold)
+  next
+    case (Seq_Step_Up \<pi> x b el \<rho>l \<kappa>l el' \<rho>l')
+
+    from H1 local.Seq_Step_Up(4) have 
+      L1H1: "is_super_exp_over_state e\<^sub>0 (\<langle>LET x = b in el;\<rho>l;\<kappa>l\<rangle>)" by blast
+
+    then have 
+      L1H2: "is_super_exp_left e\<^sub>0 (LET x = b in el)" and
+      L1H3: "is_super_exp_over_env e\<^sub>0 \<rho>l" and
+      L1H4: "is_super_exp_over_stack e\<^sub>0 \<kappa>l" by (blast dest: is_super_exp_over_state.cases)+
+
+    from L1H2 have 
+      L1H5: "is_super_exp_left e\<^sub>0 el" by (blast dest: is_super_exp_left.Let)
+
+    from L1H3 L1H4 L1H5 have 
+      L1H6: "is_super_exp_over_stack e\<^sub>0 (\<langle>x,el,\<rho>l\<rangle> # \<kappa>l)" 
+        by (simp add: is_super_exp_over_stack.Nonempty)
+
+    from local.Seq_Step_Up(5)
+    have 
+      L1H7: "is_super_exp_left e\<^sub>0 el' \<and> is_super_exp_over_env e\<^sub>0 \<rho>l'"
+    proof cases
+      case (Let_Case_Left x\<^sub>s x\<^sub>l' \<rho>\<^sub>l \<omega>\<^sub>l x\<^sub>l x\<^sub>r e\<^sub>r)
+
+      from L1H2 local.Let_Case_Left(1) have 
+        L2H1: "is_super_exp_left e\<^sub>0 el'" by (blast dest: is_super_exp_left.Let_Case_Left)
+
+      from L1H3 local.Let_Case_Left(3) have 
+        "is_super_exp_over_val e\<^sub>0 (VClosure (prim.Left x\<^sub>l') \<rho>\<^sub>l)"
+        by (blast dest: is_super_exp_over_env.cases)
+
+      then have "is_super_exp_over_env e\<^sub>0 \<rho>\<^sub>l" by (blast dest: is_super_exp_over_val.cases)
+
+      with local.Let_Case_Left(4) have "is_super_exp_over_val e\<^sub>0 \<omega>\<^sub>l" by (blast dest: is_super_exp_over_env.cases)
+
+      with L1H3 have "is_super_exp_over_env e\<^sub>0 (\<rho>l(x\<^sub>l \<mapsto> \<omega>\<^sub>l))"
+        by (smt is_super_exp_over_env.cases is_super_exp_over_env_is_super_exp_over_val.Intro map_upd_Some_unfold)
+
+      with local.Let_Case_Left(2) have 
+        L2H2: "is_super_exp_over_env e\<^sub>0 \<rho>l'" by simp
+
+      with L2H1 show "is_super_exp_left e\<^sub>0 el' \<and> is_super_exp_over_env e\<^sub>0 \<rho>l'" by simp
+    next
+      case (Let_Case_Right x\<^sub>s x\<^sub>r' \<rho>\<^sub>r \<omega>\<^sub>r x\<^sub>l e\<^sub>l x\<^sub>r)
+
+      from L1H2 local.Let_Case_Right(1) have 
+        L2H1: "is_super_exp_left e\<^sub>0 el'"
+          by (blast dest: is_super_exp_left.Let_Case_Right)
+
+      from L1H3 local.Let_Case_Right(3)
+      have "is_super_exp_over_val e\<^sub>0 (VClosure (prim.Right x\<^sub>r') \<rho>\<^sub>r)"
+        by (blast dest: is_super_exp_over_env.cases)
+
+      then have "is_super_exp_over_env e\<^sub>0 \<rho>\<^sub>r" by (blast dest: is_super_exp_over_val.cases)
+
+      with L1H3 local.Let_Case_Right(2) local.Let_Case_Right(4) have 
+        L2H2: "is_super_exp_over_env e\<^sub>0 \<rho>l'"
+          by (auto simp: is_super_exp_over_env.simps)
+
+      with L2H1 show "is_super_exp_left e\<^sub>0 el' \<and> is_super_exp_over_env e\<^sub>0 \<rho>l'" by simp
+    next
+      case (Let_App f f\<^sub>l x\<^sub>l \<rho>\<^sub>l x\<^sub>a \<omega>\<^sub>a)
+
+      from L1H3 local.Let_App(3) have
+        L2H1: "is_super_exp_over_val e\<^sub>0 (VClosure (Abs f\<^sub>l x\<^sub>l el') \<rho>\<^sub>l)" by (blast dest: is_super_exp_over_env.cases)
+
+      then have 
+        "is_super_exp_over_prim e\<^sub>0 (Abs f\<^sub>l x\<^sub>l el')" by (blast dest: is_super_exp_over_val.cases)
+
+      then have L2H2: "is_super_exp_left e\<^sub>0 el'" by (blast dest: is_super_exp_over_prim.cases)
+
+      from L2H1 have L2H3: "is_super_exp_over_env e\<^sub>0 \<rho>\<^sub>l" by (blast dest: is_super_exp_over_val.cases)
+
+      with L1H3 local.Let_App(4) have
+        L2H1: "is_super_exp_over_val e\<^sub>0 \<omega>\<^sub>a" by (blast dest: is_super_exp_over_env.cases)
+
+      with L1H3 L2H3 local.Let_App(2) local.Let_App(3) have 
+        L2H4: "is_super_exp_over_env e\<^sub>0 \<rho>l'" by (auto simp: is_super_exp_over_env.simps)
+
+       with L2H2 show "is_super_exp_left e\<^sub>0 el' \<and> is_super_exp_over_env e\<^sub>0 \<rho>l'" by simp
+    qed
+
+    with L1H6 have "is_super_exp_over_state e\<^sub>0 (\<langle>el';\<rho>l';\<langle>x,el,\<rho>l\<rangle> # \<kappa>l\<rangle>)" by (simp add: is_super_exp_over_state.intros)
+
+    with H1 H2 local.Seq_Step_Up(1) show 
+      "is_super_exp_over_state e\<^sub>0 \<sigma>'" by (metis fun_upd_other fun_upd_same map_add_empty map_add_upd option.sel)
+  next
+    case (Let_Chan \<pi> x e \<rho> \<kappa>)
+
+    from H1 local.Let_Chan(4) have 
+      "is_super_exp_over_state e\<^sub>0 (\<langle>LET x = CHAN \<lparr>\<rparr> in e;\<rho>;\<kappa>\<rangle>)" by simp
+
+    then have
+      L1H1: "is_super_exp_left e\<^sub>0 (LET x = CHAN \<lparr>\<rparr> in e)" and
+      L1H2: "is_super_exp_over_env e\<^sub>0 \<rho>" and
+      L1H3: "is_super_exp_over_stack e\<^sub>0 \<kappa>" using is_super_exp_over_state.cases by blast+
+
+    from L1H1 have
+      L1H4: "is_super_exp_left e\<^sub>0 e" using is_super_exp_left.Let by blast
+
+    from L1H2 have
+      L1H5: "is_super_exp_over_env e\<^sub>0 (\<rho>(x \<mapsto> VChan (Ch \<pi> x)))" using VChan is_super_exp_over_env.simps by auto
+
+    from L1H4 L1H5 L1H3 have
+      "is_super_exp_over_state e\<^sub>0 (\<langle>e;\<rho> ++ [x \<mapsto> VChan (Ch \<pi> x)];\<kappa>\<rangle>)" using is_super_exp_over_state.intros by simp
+
+    with H1 H2 local.Let_Chan(1) show
+      "is_super_exp_over_state e\<^sub>0 \<sigma>'" by (metis fun_upd_other fun_upd_same map_add_empty map_add_upd option.sel)
+  next
+    case (Let_Spawn \<pi> x e\<^sub>c e \<rho> \<kappa>)
+
+    from H1 local.Let_Spawn(4) have
+      "is_super_exp_over_state e\<^sub>0 (\<langle>LET x = SPAWN e\<^sub>c in e;\<rho>;\<kappa>\<rangle>)" by blast
+
+    then have
+      L1H1: "is_super_exp_left e\<^sub>0 (LET x = SPAWN e\<^sub>c in e)" and
+      L1H2: "is_super_exp_over_env e\<^sub>0 \<rho>" and
+      L1H3: "is_super_exp_over_stack e\<^sub>0 \<kappa>" using is_super_exp_over_state.cases by blast+
+
+    from L1H1 have
+      L1H4: "is_super_exp_left e\<^sub>0 e\<^sub>c" using is_super_exp_left.Let_Spawn_Child by blast
+
+    from L1H1 have
+      L1H5: "is_super_exp_left e\<^sub>0 e" using is_super_exp_left.Let by blast
+
+    from L1H2 L1H4 have
+      L1H6: "is_super_exp_over_state e\<^sub>0 (\<langle>e\<^sub>c;\<rho>;[]\<rangle>)" by (simp add: is_super_exp_over_stack.Empty is_super_exp_over_state.intros)
+
+    have
+      L1H7: "is_super_exp_over_val e\<^sub>0 VUnit" by (simp add: VUnit)
+
+    from L1H2 L1H3 L1H5 L1H7 have
+      L1H8: "is_super_exp_over_state e\<^sub>0 (\<langle>e;\<rho>(x \<mapsto> VUnit);\<kappa>\<rangle>)" by (simp add:is_super_exp_over_env.simps is_super_exp_over_state.intros)
+   
+    from H1 H2 L1H6 L1H8 local.Let_Spawn(1) show
+      "is_super_exp_over_state e\<^sub>0 \<sigma>'" by (smt fun_upd_apply map_add_empty map_add_upd option.sel)
+
+  next
+    case (Let_Sync \<pi>\<^sub>s x\<^sub>s x\<^sub>s\<^sub>e e\<^sub>s \<rho>\<^sub>s \<kappa>\<^sub>s x\<^sub>s\<^sub>c x\<^sub>m \<rho>\<^sub>s\<^sub>e \<pi>\<^sub>r x\<^sub>r x\<^sub>r\<^sub>e e\<^sub>r \<rho>\<^sub>r \<kappa>\<^sub>r x\<^sub>r\<^sub>c \<rho>\<^sub>r\<^sub>e c \<omega>\<^sub>m)
+
+    from H1 local.Let_Sync(7) have 
+      "is_super_exp_over_state e\<^sub>0 (\<langle>LET x\<^sub>r = SYNC x\<^sub>r\<^sub>e in e\<^sub>r;\<rho>\<^sub>r;\<kappa>\<^sub>r\<rangle>)" by blast
+
+    then have 
+      L1H1: "is_super_exp_left e\<^sub>0 (LET x\<^sub>r = SYNC x\<^sub>r\<^sub>e in e\<^sub>r)" and
+      L1H2: "is_super_exp_over_env e\<^sub>0 \<rho>\<^sub>r" and
+      L1H3: "is_super_exp_over_stack e\<^sub>0 \<kappa>\<^sub>r" using is_super_exp_over_state.cases by blast+
+
+    have 
+      L1H4: "is_super_exp_left e\<^sub>0 e\<^sub>r"
+      using L1H1 is_super_exp_left.Let by blast
+
+    from H1 local.Let_Sync(4) have 
+      "is_super_exp_over_state e\<^sub>0 (\<langle>LET x\<^sub>s = SYNC x\<^sub>s\<^sub>e in e\<^sub>s;\<rho>\<^sub>s;\<kappa>\<^sub>s\<rangle>)" by blast
+
+    then have 
+      L1H5: "is_super_exp_left e\<^sub>0 (LET x\<^sub>s = SYNC x\<^sub>s\<^sub>e in e\<^sub>s)" and
+      L1H6: "is_super_exp_over_env e\<^sub>0 \<rho>\<^sub>s" and
+      L1H7: "is_super_exp_over_stack e\<^sub>0 \<kappa>\<^sub>s" using is_super_exp_over_state.cases by blast+
+
+    from L1H6 local.Let_Sync(5) have 
+      L1H8: "is_super_exp_over_val e\<^sub>0 (VClosure (Send_Evt x\<^sub>s\<^sub>c x\<^sub>m) \<rho>\<^sub>s\<^sub>e)" using is_super_exp_over_env.cases by auto
+
+    then have 
+      L1H9: "is_super_exp_over_env e\<^sub>0 \<rho>\<^sub>s\<^sub>e"  using is_super_exp_over_val.cases by blast
+
+    from L1H9 local.Let_Sync(11) have 
+      L1H10: "is_super_exp_over_val e\<^sub>0 \<omega>\<^sub>m" using is_super_exp_over_env.cases by auto
+
+    from L1H5 have 
+      L1H11: "is_super_exp_left e\<^sub>0 e\<^sub>s" using is_super_exp_left.Let by blast
+
+    have 
+      L1H12: "is_super_exp_over_val e\<^sub>0 VUnit" by (simp add: VUnit)
+
+    from L1H2 L1H3 L1H4 L1H10 L1H12 have 
+      L1H13: "is_super_exp_over_state e\<^sub>0 (\<langle>e\<^sub>r;\<rho>\<^sub>r(x\<^sub>r \<mapsto> \<omega>\<^sub>m);\<kappa>\<^sub>r\<rangle>)" by (simp add: is_super_exp_over_env.simps is_super_exp_over_state.intros)
+
+    from L1H6 L1H7 L1H11 L1H12 have 
+      L1H14: "is_super_exp_over_state e\<^sub>0 (\<langle>e\<^sub>s;\<rho>\<^sub>s(x\<^sub>s \<mapsto> VUnit);\<kappa>\<^sub>s\<rangle>)" by (simp add: is_super_exp_over_env.simps is_super_exp_over_state.intros)
+
+    from H1 H2 L1H13 L1H14 local.Let_Sync(1) show 
+      "is_super_exp_over_state e\<^sub>0 \<sigma>'" by (smt fun_upd_apply map_add_empty map_add_upd option.sel)
+
+  qed
+qed
+
+lemma isnt_exp_sound_generalized: "
+  (\<E>0, H0) \<rightarrow>* (\<E>', H') \<Longrightarrow>
+  \<E>0 = [[] \<mapsto> \<langle>e\<^sub>0;Map.empty;[]\<rangle>] \<Longrightarrow>
+  \<E>' \<pi>' = Some \<sigma>' \<Longrightarrow>
+  is_super_exp_over_state e\<^sub>0 \<sigma>'
+"
+proof -
+  assume 
+    H1: "\<E>0 = [[] \<mapsto> \<langle>e\<^sub>0;Map.empty;[]\<rangle>]" and 
+    H2: "\<E>' \<pi>' = Some \<sigma>'" and
+    H3: "(\<E>0, H0) \<rightarrow>* (\<E>', H')"
+
+  obtain X0 X' where
+    H4: "X0 = (\<E>0, H0)" and 
+    H5: "X' = (\<E>', H')" by simp
+
+  from H3 H4 H5 have 
+    H6: "star_left (op \<rightarrow>) X0 X'" by (simp add: star_implies_star_left)
+
+  then have 
+    H7: "
+      \<forall> \<E>0 H0 \<E>' H' \<pi>' \<sigma>' .
+      X0 = (\<E>0, H0) \<longrightarrow> X' = (\<E>', H') \<longrightarrow>
+      \<E>0 = [[] \<mapsto> \<langle>e\<^sub>0;Map.empty;[]\<rangle>] \<longrightarrow>
+      \<E>' \<pi>' = Some \<sigma>' \<longrightarrow>
+      is_super_exp_over_state e\<^sub>0 \<sigma>'
+    " 
+  proof (induction)
+    case (refl z)
+
+    {
+      fix \<E>0 H0 \<E>' H' \<pi>' \<sigma>'
+      assume 
+        L1H0: "z = (\<E>0, H0)" "z = (\<E>', H')" and
+        L1H1: "\<E>0 = [[] \<mapsto> \<langle>e\<^sub>0;Map.empty;[]\<rangle>]" and
+        L1H2:  "\<E>0 \<pi>' = Some \<sigma>'"
+  
+      have 
+        L1H3: "is_super_exp_left e\<^sub>0 e\<^sub>0" by (simp add: is_super_exp_left.Refl)
+      have 
+        L1H4: "is_super_exp_over_env e\<^sub>0 Map.empty" by (simp add: is_super_exp_over_env_is_super_exp_over_val.Intro)
+      have 
+        L1H5: "is_super_exp_over_stack e\<^sub>0 []" by (simp add: is_super_exp_over_stack.Empty)
+
+      from L1H3 L1H4 L1H5 have 
+        L1H6: "is_super_exp_over_state e\<^sub>0 (\<langle>e\<^sub>0;Map.empty;[]\<rangle>)" by (simp add: is_super_exp_over_state.intros)
+
+     from L1H1 L1H2 L1H6 have
+        "is_super_exp_over_state e\<^sub>0 \<sigma>'" by (metis fun_upd_apply option.distinct(1) option.sel)
+    }
+
+    then show ?case by blast
+  next
+    case (step x y z)
+    {
+      fix \<E>0 H0 \<E>' H' \<pi>' \<sigma>'
+      assume 
+        L1H0: "x = (\<E>0, H0)" "z = (\<E>', H')" and 
+        L2H1: "\<E>0 = [[] \<mapsto> \<langle>e\<^sub>0;Map.empty;[]\<rangle>]" and
+        L2H2: "\<E>' \<pi>' = Some \<sigma>'"
+
+
+      obtain \<E> H where L2H3: "y = (\<E>, H)" by (meson surj_pair)
+      from L1H0(1) L2H1 L2H3 step.IH have 
+        L2H4: "\<forall>\<pi> \<sigma>. \<E> \<pi> = Some \<sigma> \<longrightarrow> is_super_exp_over_state e\<^sub>0 \<sigma>" by blast
+
+      from L1H0(2) L2H2 L2H3 L2H4 step.hyps(2) have 
+        "is_super_exp_over_state e\<^sub>0 \<sigma>'" using is_super_exp_over_state_preserved by blast
+
+    } 
+
+    then show ?case by blast
+  qed
+
+  from H1 H2 H4 H5 H7 show 
+    "is_super_exp_over_state e\<^sub>0 \<sigma>'" by blast
+qed
+
+lemma isnt_exp_sound: "
+  ([[] \<mapsto> \<langle>e\<^sub>0;Map.empty;[]\<rangle>], {}) \<rightarrow>* (\<E>', H') \<Longrightarrow>
+  \<E>' \<pi>' = Some (\<langle>e';\<rho>';\<kappa>'\<rangle>) \<Longrightarrow>
+  is_super_exp e\<^sub>0 e'
+" 
+using is_super_exp_left_implies_is_super_exp is_super_exp_over_state.simps isnt_exp_sound_generalized by fastforce
+
 
 
 end
